simulate: use a stack without dependent types

RocqOfRust/simulate/M.v
@@ -2,116 +2,122 @@ Require Import RocqOfRust.RocqOfRust.
 Require Import links.M.
 
 Module Stack.
-  Definition t : Type :=
-    list Set.
+  Inductive t : Set :=
+  | Nil
+  | Cons {A : Set} (value : A) (stack : t).
 
-  Fixpoint to_Set (Stack : t) : Set :=
-    match Stack with
-    | [] => unit
-    | A :: Stack => A * to_Set Stack
+  Module Nth.
+    Inductive t (A : Set) : Stack.t -> nat -> Set :=
+    | ConsZero (value : A) (stack : Stack.t) :
+      t A (Stack.Cons value stack) 0
+    | ConsSucc {A' : Set} (value : A') (stack : Stack.t) (index : nat) :
+      t A stack index ->
+      t A (Stack.Cons value stack) (S index).
+  End Nth.
+
+  Fixpoint length (stack : t) : nat :=
+    match stack with
+    | Nil => 0
+    | Cons _ stack => S (length stack)
     end.
 
-  Definition nth (Stack : t) (index : nat) : Set :=
-    List.nth index Stack unit.
-
-  Fixpoint read {Stack : t}
-    (stack : to_Set Stack)
-    (index : nat)
-    {struct Stack} :
-    nth Stack index.
+  Fixpoint read
+    {stack : t} {index : nat} {A : Set}
+    (nth : Nth.t A stack index)
+    {struct nth} :
+    A.
   Proof.
-    destruct Stack as [|A Stack], index as [|index]; cbn in *.
-    { exact tt. }
-    { exact tt. }
-    { exact (fst stack). }
-    { exact (read _ (snd stack) index). }
+    destruct nth.
+    { exact value. }
+    { exact (read _ _ _ nth). }
   Defined.
 
-  Fixpoint write {Stack : t}
-    (stack : to_Set Stack)
-    (index : nat)
-    (value : nth Stack index)
-    {struct Stack} :
-    to_Set Stack.
+  Fixpoint write
+    {stack : t} {index : nat} {A : Set}
+    (nth : Nth.t A stack index)
+    (new_value : A)
+    {struct nth} :
+    t.
   Proof.
-    destruct Stack as [|A Stack], index as [|index]; cbn in *.
-    { exact tt. }
-    { exact tt. }
-    { exact (value, snd stack). }
-    { exact (fst stack, write _ (snd stack) index value). }
+    destruct nth.
+    { exact (Cons new_value stack). }
+    { exact (Cons value (write _ _ _ nth new_value)). }
   Defined.
 
-  Fixpoint alloc {Stack : t} {A : Set}
-    (stack : to_Set Stack)
-    (value : A)
-    {struct Stack} :
-    to_Set (Stack ++ [A]).
+  Fixpoint alloc {A : Set}
+    (stack : t)
+    (new_value : A)
+    {struct stack} :
+    t.
   Proof.
-    destruct Stack as [|A' Stack]; cbn in *.
-    { exact (value, tt). }
-    { exact (fst stack, alloc _ _ (snd stack) value). }
+    destruct stack.
+    { exact (Cons new_value Nil). }
+    { exact (Cons value (alloc _ stack new_value)). }
   Defined.
+  Arguments alloc _ _ /.
 
-  Fixpoint dealloc {Stack : t} {A : Set}
-    (stack : to_Set (Stack ++ [A]))
-    {struct Stack} :
-    to_Set Stack * A.
-  Proof.
-    destruct Stack as [|A' Stack]; cbn in *.
-    { exact (tt, fst stack). }
-    { exact (
-        let '(stack', value) := dealloc _ _ (snd stack) in
-        ((fst stack, stack'), value)
-      ).
-    }
-  Defined.
+  Fixpoint dealloc (stack : t) {struct stack} : t :=
+    match stack with
+    | Nil => Nil
+    | Cons _ Nil => Nil
+    | Cons value stack => Cons value (dealloc stack)
+    end.
+
+  Declare Scope stack_scope.
+  Delimit Scope stack_scope with stack.
+
+  Notation "[ ]" := Nil (format "[ ]") : stack_scope.
+  Notation "[ x ]" := (Cons x Nil) (format "[ x ]") : stack_scope.
+  Notation "[ x ; y ; .. ; z ]" := (Cons x (Cons y .. (Cons z Nil) ..)) (format "[ x ; y ; .. ; z ]") : stack_scope.
+  Notation "x :: y" := (Cons x y) (at level 60, right associativity) : stack_scope.
 
   Module CanAccess.
-    Inductive t {A : Set} `{Link A} (Stack : Stack.t) : Ref.Core.t A -> Set :=
+    Inductive t {A : Set} `{Link A} (stack : Stack.t) : Ref.Core.t A -> Set :=
     | Mutable
-        (index : nat)
+        (index : nat) (Big_A : Set)
+        (nth : Nth.t Big_A stack index)
         (path : Pointer.Path.t)
-        (big_to_value : nth Stack index -> Value.t)
-        (projection : nth Stack index -> option A)
-        (injection : nth Stack index -> A -> option (nth Stack index)) :
-      t Stack (Ref.Core.Mutable (Address := nat) (Big_A := nth Stack index)
+        (big_to_value : Big_A -> Value.t)
+        (projection : Big_A -> option A)
+        (injection : Big_A -> A -> option Big_A) :
+      t stack (Ref.Core.Mutable (Address := nat) (Big_A := Big_A)
         index path big_to_value projection injection
       ).
 
-    Definition runner {Stack : Stack.t} {A : Set} `{Link A} {index : Pointer.Index.t}
+    Definition runner {stack : Stack.t} {A : Set} `{Link A} {index : Pointer.Index.t}
         {ref_core : Ref.Core.t A}
         (runner : SubPointer.Runner.t A index)
-        (H_ref_core : t Stack ref_core) :
-      t Stack (SubPointer.Runner.apply ref_core runner).
+        (H_ref_core : t stack ref_core) :
+      t stack (SubPointer.Runner.apply ref_core runner).
     Proof.
       destruct H_ref_core.
       apply Mutable.
+      exact nth.
     Defined.
 
-    Definition read {A : Set} `{Link A} {Stack : Stack.t}
+    Definition read {A : Set} `{Link A} {stack : Stack.t}
         {ref_core : Ref.Core.t A}
-        (run : t Stack ref_core)
-        (stack : to_Set Stack) :
+        (run : t stack ref_core) :
         option A :=
       match run with
-      | Mutable _ index _ _ projection _ => projection (read stack index)
+      | Mutable _ _ _ nth _ _ projection _ => projection (read nth)
       end.
 
-    Definition write {A : Set} `{Link A} {Stack : Stack.t}
+    Definition write {A : Set} `{Link A} {stack : Stack.t}
         {ref_core : Ref.Core.t A}
-        (run : t Stack ref_core)
-        (stack : to_Set Stack)
+        (run : t stack ref_core)
         (value : A) :
-        option (to_Set Stack) :=
+        option Stack.t :=
       match run with
-      | Mutable _ index _ _ _ injection =>
-        match injection (Stack.read stack index) value with
-        | Some value => Some (Stack.write stack index value)
+      | Mutable _ _ _ nth _ _ _ injection =>
+        match injection (Stack.read nth) value with
+        | Some value => Some (Stack.write nth value)
         | None => None
         end
       end.
   End CanAccess.
 End Stack.
+Export (notations) Stack.
 
 (** Here we define an execution mode where we keep dynamic cast to retrieve data from the stack. In
     practice, these casts should always be correct as the original Rust code was well typed. *)
@@ -119,17 +125,17 @@ Module SimulateM.
   Inductive t (A : Set) : Set :=
   | Pure (value : A)
   | GetCanAccess {B : Set} `{Link B}
-      (Stack : Stack.t)
+      (stack : Stack.t)
       (ref_core : Ref.Core.t B)
-      (k : Stack.CanAccess.t Stack ref_core -> t A)
-  | Call {B : Set} `{Link B} {Stack : Stack.t}
+      (k : Stack.CanAccess.t stack ref_core -> t A)
+  | Call {B : Set} `{Link B}
       {f : list Value.t -> M} {args : list Value.t}
-      (stack_in : Stack.to_Set Stack)
+      (stack_in : Stack.t)
       (run_f : {{ f args 🔽 B }})
-      (k : Output.t B B * Stack.to_Set Stack -> t A).
+      (k : Output.t B B * Stack.t -> t A).
   Arguments Pure {_}.
   Arguments GetCanAccess {_ _ _}.
-  Arguments Call {_ _ _ _ _ _}.
+  Arguments Call {_ _ _ _ _}.
 
   Fixpoint let_ {A B : Set} (e1 : t A) (e2 : A -> t B) : t B :=
     match e1 with
@@ -143,8 +149,8 @@ Module SimulateM.
     (let_ X (fun x => Y))
     (at level 200, x pattern, X at level 100, Y at level 200).
 
-  Definition read {R : Set} {Stack : Stack.t} {A : Set} `{Link A}
-      (stack : Stack.to_Set Stack)
+  Definition read {R : Set} {A : Set} `{Link A}
+      (stack : Stack.t)
       (ref_core : Ref.Core.t A) :
       t (Output.t R A) :=
     match ref_core with
@@ -154,8 +160,8 @@ Module SimulateM.
       | None => Pure (Output.Exception Output.Exception.BreakMatch)
       end
     | Ref.Core.Mutable _ _ _ _ _ =>
-      GetCanAccess Stack ref_core (fun H_can_access =>
-      match Stack.CanAccess.read H_can_access stack with
+      GetCanAccess stack ref_core (fun H_can_access =>
+      match Stack.CanAccess.read H_can_access with
       | Some value => Pure (Output.Success value)
       | None => Pure (Output.Exception Output.Exception.BreakMatch)
       end)
@@ -163,11 +169,11 @@ Module SimulateM.
 
   Parameter TodoLoop : forall {A : Set}, t A.
 
-  Fixpoint eval {R Output : Set} {Stack : Stack.t}
+  Fixpoint eval {R Output : Set}
       (e : LinkM.t R Output)
-      (stack : Stack.to_Set Stack)
+      (stack : Stack.t)
       {struct e} :
-    t (Output.t R Output * Stack.to_Set Stack).
+    t (Output.t R Output * Stack.t).
   Proof.
     destruct e.
     { (* Pure *)
@@ -177,14 +183,14 @@ Module SimulateM.
       destruct primitive.
       { (* StateAlloc *)
         (* We always allocate an immediate value *)
-        exact (eval _ _ _ (k (Ref.Core.Immediate (Some value))) stack).
+        exact (eval _ _ (k (Ref.Core.Immediate (Some value))) stack).
       }
       { (* StateRead *)
         exact (
           let_ (read stack ref_core) (fun value =>
           match value with
           | Output.Success value =>
-            eval _ _ _ (k value) stack
+            eval _ _ (k value) stack
           | Output.Exception exception =>
             Pure (Output.Exception exception, stack)
           end)
@@ -192,48 +198,48 @@ Module SimulateM.
       }
       { (* StateWrite *)
         refine (
-          GetCanAccess Stack ref_core (fun H_access =>
+          GetCanAccess stack ref_core (fun H_access =>
           _)
         ).
-        destruct (Stack.CanAccess.write H_access stack value) as [stack'|].
-        { exact (eval _ _ _ (k tt) stack'). }
+        destruct (Stack.CanAccess.write H_access value) as [stack'|].
+        { exact (eval _ _ (k tt) stack'). }
         { exact (Pure (Output.panic "StateWrite: invalid reference", stack)). }
       }
       { (* GetSubPointer *)
-        exact (eval _ _ _ (k (SubPointer.Runner.apply ref_core runner)) stack).
+        exact (eval _ _ (k (SubPointer.Runner.apply ref_core runner)) stack).
       }
     }
     { (* Let *)
       exact (
-        let_ (eval _ _ _ e stack) (fun '(output, stack) =>
-        eval _ _ _ (k output) stack)
+        let_ (eval _ _ e stack) (fun '(output, stack) =>
+        eval _ _ (k output) stack)
       ).
     }
     { (* LetAlloc *)
       exact (
-        let_ (eval _ _ _ e stack) (fun '(output, stack) =>
+        let_ (eval _ _ e stack) (fun '(output, stack) =>
         match output with
         | Output.Success value =>
           let ref_core :=
             Ref.Core.Mutable
-              (List.length Stack)
+              (Stack.length stack)
               []
               φ
               Some
               (fun _ => Some) in
           let ref := {| Ref.core := ref_core |} in
           let stack := Stack.alloc stack value in
-          let_ (eval _ _ _ (k (Output.Success ref)) stack) (fun '(output, stack) =>
-          let '(stack, _) := Stack.dealloc stack in
+          let_ (eval _ _ (k (Output.Success ref)) stack) (fun '(output, stack) =>
+          let stack := Stack.dealloc stack in
           Pure (output, stack))
-        | Output.Exception exception => eval _ _ _ (k (Output.Exception exception)) stack
+        | Output.Exception exception => eval _ _ (k (Output.Exception exception)) stack
         end)
       ).
     }
     { (* Call *)
       exact (Call stack run_f0 (fun '(output, stack) =>
         SuccessOrPanic.apply (fun output =>
-          eval _ _ _ (k output) stack
+          eval _ _ (k output) stack
         ) output
       )).
     }
@@ -243,22 +249,22 @@ Module SimulateM.
     { (* IfThenElse *)
       exact (
         if cond then
-          eval _ _ _ e1 stack
+          eval _ _ e1 stack
         else
-          eval _ _ _ e2 stack
+          eval _ _ e2 stack
       ).
     }
     { (* MatchOutput *)
       exact (
         match output with
-        | Output.Success success => eval _ _ _ (k_success success) stack
+        | Output.Success success => eval _ _ (k_success success) stack
         | Output.Exception exception =>
           match exception with
-          | Output.Exception.Return return_ => eval _ _ _ (k_return return_) stack
-          | Output.Exception.Break => eval _ _ _ (k_break tt) stack
-          | Output.Exception.Continue => eval _ _ _ (k_continue tt) stack
-          | Output.Exception.BreakMatch => eval _ _ _ (k_break_match tt) stack
-          | Output.Exception.Panic panic => eval _ _ _ (k_panic panic) stack
+          | Output.Exception.Return return_ => eval _ _ (k_return return_) stack
+          | Output.Exception.Break => eval _ _ (k_break tt) stack
+          | Output.Exception.Continue => eval _ _ (k_continue tt) stack
+          | Output.Exception.BreakMatch => eval _ _ (k_break_match tt) stack
+          | Output.Exception.Panic panic => eval _ _ (k_panic panic) stack
           end
         end
       ).
@@ -271,12 +277,11 @@ Module SimulateM.
       {τ : list Ty.t}
       {α : list Value.t}
       {Output : Set} `{Link Output}
-      {Stack : Stack.t}
       (run : Run.Trait f ε τ α Output) :
-      Stack.to_Set Stack ->
-      t (Output.t Output Output * Stack.to_Set Stack) :=
+      Stack.t ->
+      t (Output.t Output Output * Stack.t) :=
     eval (links.M.evaluate run.(Run.run_f)).
-  Arguments eval_f _ _ _ _ _ _ _ _ _ /.
+  Arguments eval_f _ _ _ _ _ _ _ _ /.
 End SimulateM.
 Export (notations) SimulateM.
 
@@ -287,18 +292,18 @@ Module Run.
   | Pure :
     {{ SimulateM.Pure value 🌲 value }}
   | GetCanAccess {B : Set} `{Link B}
-      (Stack : Stack.t)
+      (stack : Stack.t)
       (ref_core : Ref.Core.t B)
-      (k : Stack.CanAccess.t Stack ref_core -> SimulateM.t A)
-      (H_access : Stack.CanAccess.t Stack ref_core)
+      (k : Stack.CanAccess.t stack ref_core -> SimulateM.t A)
+      (H_access : Stack.CanAccess.t stack ref_core)
     (H_k : {{ k H_access 🌲 value }}) :
-    {{ SimulateM.GetCanAccess Stack ref_core k 🌲 value }}
-  | Call {B : Set} `{Link B} {Stack : Stack.t}
+    {{ SimulateM.GetCanAccess stack ref_core k 🌲 value }}
+  | Call {B : Set} `{Link B}
       {f : list Value.t -> M} {args : list Value.t}
-      (stack_in : Stack.to_Set Stack)
+      (stack_in : Stack.t)
       (run_f : {{ f args 🔽 B }})
-      (value_inter : Output.t B B * Stack.to_Set Stack)
-      (k : Output.t B B * Stack.to_Set Stack -> SimulateM.t A)
+      (value_inter : Output.t B B * Stack.t)
+      (k : Output.t B B * Stack.t -> SimulateM.t A)
     (H_f : {{ SimulateM.eval (links.M.evaluate run_f) stack_in 🌲 value_inter }})
     (H_k : {{ k value_inter 🌲 value }}) :
     {{ SimulateM.Call stack_in run_f k 🌲 value }}
@@ -310,10 +315,7 @@ Export (notations) Run.
 Ltac get_can_access :=
   unshelve eapply Run.GetCanAccess; [
     cbn;
-    match goal with
-    | |- Stack.CanAccess.t ?Stack (Ref.Core.Mutable ?index _ _ _ ?injection) =>
-      apply (Stack.CanAccess.Mutable Stack index _ _ _ injection)
-    end
+    repeat constructor
   |];
   cbn.
 
